# Apply example

## Status

| human  | copilot | auto   | crush  | sauto  | hammer | gpt4   |
| ---    | ---     | ---    | ---    | ---    | ---    | ---    |
| [âœ…](./human.v) | [ðŸ”„](./auto.v) | [ðŸ”„](./copilot.v) | [ðŸ”„](./crush.v) | [ðŸ”„](./gpt4.v) | [ðŸ”„](./hammer.v) | [ðŸ”„](./sauto.v) |

## Script

We want to prove the following statement:

```coq
Variables P Q R T: Prop.
Theorem apply_example: (Q -> R -> T) -> (P -> Q) -> P -> R -> T.
```

If Q and R implies T
and P implies Q
then given P and R
we should be able to show T

